new/proof/btree_proof/query.v
@@ -1,0 +1,73 @@
+From New.generatedproof Require Import btree.
+From New.proof Require Import proof_prelude.
+From New.proof.btree_proof Require Import btree_init rep items.
+
+(** * Read-only btree operations: Get, Has, Len, Min, Max. *)
+
+Section proof.
+Context `{hG: heapGS Σ, !ffi_semantics _ _} `{!globalsGS Σ} {go_ctx: GoContext}.
+
+(** ** Len *)
+
+Lemma wp_BTree__Len R (t : loc) (elems : gset interface.t) :
+  {{{ is_pkg_init btree ∗ btree_repr R t elems }}}
+    t @ (ptrT.id btree.BTree.id) @ "Len"%go #()
+  {{{ (n : w64), RET #n;
+      btree_repr R t elems ∗
+      ⌜uint.Z n = Z.of_nat (size elems)⌝ }}}.
+Proof.
+  wp_start as "H".
+  iNamed "H".
+  wp_auto.
+  iApply "HΦ".
+  iFrame. iPureIntro. done.
+Qed.
+
+(** ** node.get *)
+
+Lemma wp_node__get height R (n : loc) (elems : gset interface.t)
+    (degree : Z) (key : interface.t) :
+  {{{ is_pkg_init btree ∗
+      node_repr height R n elems degree ∗
+      is_less_order R ∗
+      ⌜key ≠ interface.nil⌝ }}}
+    n @ (ptrT.id btree.node.id) @ "get"%go #key
+  {{{ (result : interface.t), RET #result;
+      node_repr height R n elems degree ∗
+      ⌜(result ≠ interface.nil → result ∈ elems ∧ ¬R result key ∧ ¬R key result) ∧
+       (result = interface.nil → ∀ e, e ∈ elems → R e key ∨ R key e)⌝ }}}.
+Proof.
+Admitted.
+
+(** ** BTree.Get *)
+
+Lemma wp_BTree__Get R (t : loc) (elems : gset interface.t)
+    (key : interface.t) :
+  {{{ is_pkg_init btree ∗
+      btree_repr R t elems ∗
+      is_less_order R ∗
+      ⌜key ≠ interface.nil⌝ }}}
+    t @ (ptrT.id btree.BTree.id) @ "Get"%go #key
+  {{{ (result : interface.t), RET #result;
+      btree_repr R t elems ∗
+      ⌜(result ≠ interface.nil → result ∈ elems ∧ ¬R result key ∧ ¬R key result) ∧
+       (result = interface.nil → ∀ e, e ∈ elems → R e key ∨ R key e)⌝ }}}.
+Proof.
+Admitted.
+
+(** ** BTree.Has *)
+
+Lemma wp_BTree__Has R (t : loc) (elems : gset interface.t)
+    (key : interface.t) :
+  {{{ is_pkg_init btree ∗
+      btree_repr R t elems ∗
+      is_less_order R ∗
+      ⌜key ≠ interface.nil⌝ }}}
+    t @ (ptrT.id btree.BTree.id) @ "Has"%go #key
+  {{{ (b : bool), RET #b;
+      btree_repr R t elems ∗
+      ⌜b ↔ ∃ e, e ∈ elems ∧ ¬R e key ∧ ¬R key e⌝ }}}.
+Proof.
+Admitted.
+
+End proof.
